\documentclass[../main.tex]{subfiles}
\graphicspath{{\subfix{../images/}}}
\begin{document}

\subsection*{Answers - Partial fractions (page \pageref{partial fractions})}
\label{Partial fractions answers}
\begin{enumerate}[itemsep=0.7cm]
    \item 
    $\frac{x+5}{(x-3)(x+1)}=\frac{A}{x-3}+\frac{B}{x+1}$

    $A(x+1)+B(x-3)=x+5$

    Using critical value method (you don't have to, you could equate coefficients and constant if you want), we substitute in $x=3$ and $x=-1$:

    $4A=8 \Rightarrow A=2$

    $-4B=4 \Rightarrow B=-1$

    Partial fraction decomposition is $\frac{2}{x-3}-\frac{1}{x+1}$

    \item 
    $\frac{x+26}{x^3+3x-10}=\frac{x+26}{(x+5)(x-2)}$

    $\frac{x+26}{(x+5)(x-2)}=\frac{A}{x+5}+\frac{B}{x-2}$

    $x+26=A(x-2)+B(x+5)$

    Using critical value method, we substitute in $x=2$ and $x=-5$

    $2+26=0+7B \Rightarrow B=4$

    $-5+26=-7A \Rightarrow A=3$

    Giving us: $\frac{3}{x+5}+\frac{4}{x-2}$

    \item 
    $\frac{4x-8}{x^2-8x+15}=\frac{4x-8}{(x-3)(x-5)}$

    $\frac{4x-8}{(x-5)(x-3)}=\frac{A}{x-3}+\frac{B}{x-5}$

    $4x-8=A(x-5)+B(x-3)$

    Using critical value method we substitute in $x=5$ and $x=3$

    $4(3)-8=-2A \Rightarrow A=-2$

    $4(5)-8=2B \Rightarrow B=6$

    Giving us $\frac{-2}{x-3}+\frac{6}{x-5}$

    \item 
    $\frac{12x-1}{x^2+x-12}=\frac{12x-1}{(x+4)(x-3)}$

    $\frac{12x-1}{(x+4)(x-3)}=\frac{A}{x+4}+\frac{B}{x-3}$

    $12x-1=A(x-3)+B(x+4)$

    Using critical values of $x=3$ and $x=-4$:

    $12(3)-1=7B \Rightarrow B=5$

    $12(-4)-1=-7A \Rightarrow A=7$

    Giving us: $\frac{7}{x+4}+\frac{5}{x-3}$

    \item 
    $\frac{x-5}{(x-2)^2}=\frac{A}{x-2}+\frac{B}{(x-2)^2}$

    $x-5=A(x-2)+B$

    $x-5=Ax-2A+B$

    Matching coefficients and constant:

    $x$-term : $A=1$

    Constant : $-2A+B=-5 \Rightarrow B=-3$

    Giving us: $\frac{1}{x-2}-\frac{3}{(x-2)^2}$

    \item 
    $\frac{5x+4}{(x-1)(x+2)^2}=\frac{A}{x-1}+\frac{B}{(x+2)}+\frac{C}{(x+2)^2}$

    $5x+4=A(x+2)^2+B(x-1)(x+2)+C(x-1)$

    $5x+4=Ax^2+4Ax+4A+Bx^2+Bx-2B+Cx-C$

    $5x+4=(A+B)x^2+(4A+B+C)x+4A-2B-C$

    Equating coefficients and constant:

    $x^2$-term : $A+B=0$

    $x$-term : $4A+B+C=5$

    Constant : $4A-2B-C=4$

    Solving simultaneously, $A=1,B=-1, C=2$

    Giving us: $\frac{1}{x-1}-\frac{1}{x+2}+\frac{2}{(x+2)^2}$

    \item 
    $\frac{2x^2-5x+7}{(x-2)(x-1)^2}=\frac{A}{x-2}+\frac{B}{x-1}+\frac{C}{(x-1)^2}$

    $2x^2-5x+7=A(x-1)^2+B(x-2)(x-1)+C(x-2)$

    $2x^2-5x+7=Ax^2-2Ax+A+Bx^2-3Bx+2B+Cx-2C$

    $2x^2-5x+7=(A+B)x^2+(-2A-3B+C)x+A+2B-2C$

    Equating coefficients and constant:

    $x^2$-term : $A+B=2$

    $x$-term : $-2A-3B+C=-5$

    Constant : $A+2B-2C=7$

    Solving simultaneously, $A=5, B=-3, C=-4$

    Giving us: $\frac{5}{x-2}-\frac{3}{x-1}+\frac{7}{(x-1)^2}$

    \item 
    $\frac{6-x}{(1-x)(4+x^2)}=\frac{A}{1-x}+\frac{Bx+C}{4+x^2}$

    $6-x=A(4+x^2)+(Bx+C)(1-x)$

    $6-x=4A+Ax^2+Bx-Bx^2+C-Cx$

    $6-x=(A-B)x^2+(B-C)x+4A+C$

    Equating coefficients and constant:

    $x^2$-term : $A-B=0$

    $x$-term : $B-C=-1$

    Constant : $4A+C=6$

    Solving simultaneously, $A=1, B=1, C=2$

    Giving us: $\frac{1}{1-x}+\frac{x+2}{4+x^2}$

    \item 
    $\frac{5x+2}{(x+1)(x^2-4)}=\frac{A}{x+1}+\frac{Bx+C}{x^2-4}$

    $5x+2=A(x^2-4)+(Bx+C)(x+1)$

    $5x+2=Ax^2-4A+Bx^2+Bx+Cx+C$

    $5x+2=(A+B)x^2+(B+C)x-4A+C$

    Equating coefficients and constant:

    $x^2$-term : $A+B=0$

    $x$-term : $B+C=5$

    Constant : $-4A+C=2$

    Solving simultaneously, $A=1, B=-1, C=6$

    Giving us: $\frac{1}{x+1}+\frac{-x+6}{x^2-4}$

\end{enumerate}




\end{document}