\documentclass[../main.tex]{subfiles}
\graphicspath{{\subfix{../images/}}}
\begin{document}
\subsection*{Answers - Euler's Formula (page \pageref{eulersformula})}
\label{Eulers answers}
\begin{spacing}{1.5}
\begin{enumerate}
    \item 
    \((-i)^i=e^{-\frac{i\pi}{2}^{i}}\\
    =e^{-\frac{i^2 \pi}{2}}\\
    =e^{\frac{\pi}{2}}\)

    \item 
    Since \(-1=e^{i \pi}\), we can write this expression as \(\ln{(e^{i \pi})}=i \pi\)

    \item 
    \(e^{i(A-B)}=e^{iA}e^{-iB}\)

    This means that:

    $
    \!
    \begin{aligned}[t]
    \cos{(A-B)+i\sin{(A-B)}}
    &=(\cos{(A)+i\sin{(A)}})(\cos{(-B)+i\sin{(-B)}})\\
    &=(\cos{(A)+i\sin{(A)}})(\cos{(B)-i\sin{(B)}})
    \end{aligned}\\
    $
    
    Equating real and imaginary parts:

    $
    \!
    \begin{aligned}[t]
    \cos{(A-B)}
    &=\cos{(A)}\cos{(B)}+\sin{(A)}\sin{(B)}\\
    \sin(A-B)
    &=\cos{(B)}\sin{(A)}-\cos{(A)}\sin{(B)}\\
    \end{aligned}\\
    $

    Substituting \(-B\) for \(B\) in the second equation:

    \(\sin{(A+B)}=\sin{(A)}\cos{(-B)}-\cos{(A)}\sin{(-B)}=\sin{(A)}\cos{(B)}+\cos{(A)}\sin{(B)}\)

    \item 
    Since \(i=e^{\frac{i \pi}{2}}\), we can write the expression as \(((e^{\frac{i \pi}{2}})^i)^2=(e^{-\frac{\pi}{2}})^2=e^{-\pi}\)

    \item 
    Separating the expression into three terms:

    \(\ln{(-25e^{i^{i}})}=\ln(-1)+\ln(25)+\ln(e^{i^{i}})\)

    Since \(-1=e^{i \pi}\), we can simplify the expression:

    \(\ln(e^{i \pi})+\ln(25)+\ln{e^{i^{i}}}\\
    i \pi + \ln(25) + i^i\)

    \(i^i=e^{\frac{i \pi}{2}^{i}}=e^{-\frac{\pi}{2}}\)

    So the expression simplifies to \(i \pi + \ln(25) + e^{-\frac{\pi}{2}}\)
    
    \item 
    \(e^{i\theta}=\cos{\theta}+i\sin{\theta}\)

    \(e^{-i\theta}=\cos{(-\theta)}+i\sin{(-\theta)}=\cos{\theta}-i\sin{\theta}\)

    \(\therefore e^{i\theta}+e^{-i\theta}=2\cos{\theta}\)

    \(\therefore \cos{\theta}=\frac{1}{2}(e^{i\theta}+e^{-i\theta})\)
    As required

    \item 
    \(e^{i\theta}=\cos{\theta}+i\sin{\theta}\)

    \(e^{-i\theta}=\cos{(-\theta)}+i\sin{(-\theta)}=\cos{\theta}-i\sin{\theta}\)

    \(\therefore e^{i\theta}-e^{-i\theta}=2i\sin{\theta}\)

    \(\therefore \sin{\theta}=\frac{1}{2i}(e^{i\theta}-e^{-i\theta})\)
    As required

    \item 
    \(\cos{\theta}=\frac{1}{2}(e^{i\theta}+e^{-i\theta})\)

    \(\therefore \cos{(i)}=\frac{1}{2}(e^{i^2}+e^{-i^2})=\frac{1}{2}(e^{-1}+e^{1})=\frac{1}{2e}+\frac{e}{2}\)

    \item 
    \(\frac{1}{2}(\sqrt{3}+i)=\cos{\frac{\pi}{6}}+i\sin{\frac{\pi}{6}}=e^{\frac{i\pi}{6}}\)

    \(\therefore -i\ln{\Bigl(\frac{1}{2}(\sqrt{3}+i)\Bigr)} = -i\ln{\Bigl(e^{\frac{i\pi}{6}}\Bigr)}\)

    \(-i \times \frac{i\pi}{6}=\frac{\pi}{6}\)

    \item 
    
    Multiply by $e^x$
    
    $e^{2x}+e^{0}=0$

    $e^{2x}+1=0$

    $e^{2x}=-1$

    $\ln{e^{2x}}=\ln{(-1)}$

    $2x=\ln{(e^{i(\pi +2n\pi)})}$

    $2x=i(\pi + 2n\pi)$

    $x=\frac{i}{2}(\pi + 2n\pi)$

\end{enumerate}
\end{spacing}
\end{document}