\documentclass[../main.tex]{subfiles}
\graphicspath{{\subfix{../images/}}}
\begin{document}
\hypertarget{implicitdiffanswers}{\subsection*{Answers - Implicit differentiation (\hyperlink{implicitdifflink}{page \pageref{Implicit Differentiation}})}}

\label{Implicit differentiation answers}
\begin{spacing}{1.5}
\begin{enumerate}
    \item
    $
    \!
    \begin{aligned}[t]
        8x + 4y\times\frac{dy}{dx}
        &= 0 \\
        4y\times\frac{dy}{dx}
        &=-8x\\
        \frac{dy}{dx}
        &=\frac{-2x}{y}
    \end{aligned}
    $
    \item 
    $
    \!
    \begin{aligned}[t]
        6y^2+12xy\times\frac{dy}{dx}-3\frac{dy}{dx}
        &=0\\
        (12xy-3)\frac{dy}{dx}
        &=-6y^2\\
        \frac{dy}{dx}
        &=\frac{-2y^2}{4xy-1}
    \end{aligned}
    $
    \item 
    $
    \!
    \begin{aligned}[t]
        10xy^2+10x^2y\frac{dy}{dx}-3y-3x\frac{dy}{dx}
        &=0\\
        (10x^2y-3x)\frac{dy}{dx}
        &=3y-10xy^2\\
        \frac{dy}{dx}
        &=\frac{3y-10xy^2}{10x^2y-3x}
    \end{aligned}
    $
    \item 
    \(y+x\frac{dy}{dx}+e^y\frac{dy}{dx}=2\)

    \(\frac{dy}{dx}=\frac{2-y}{x+e^y} \) 

    \(\frac{d^2y}{dx^2}=\frac{-(x+e^y)\frac{dy}{dx}-(2-y)(1+e^y\frac{dy}{dx})}{(x+e^y)^2}\)

    When \(x=0, e^y=1\Rightarrow{}y=0\text{ and }\frac{dy}{dx}=\frac{2-0}{0+1}=2\)

    Hence,

    $
    \!
    \begin{aligned}[t]
        \frac{d^2y}{dx^2}
        &=\frac{-(x+e^y)\frac{dy}{dx}-(2-y)(1+e^y\frac{dy}{dx})}{(x+e^y)^2}\\
        &=\frac{-(0+1)2-(2-0)(1+2\times2)}{(0+1)^2}\\
        &=-8\\
    \end{aligned}
    $
    \item 
    
    $
    \text{Let} y=\sinh^{-1}{x}\Rightarrow{}\sinh{y}=x\\
    x=\frac{1}{2}(e^y-e^{-y})\Rightarrow{}\\
    \text{Differentiating implicitly:}\\
    1=\frac{1}{2}(e^y\frac{dy}{dx}+e^{-y}\frac{dy}{dx})\\
    \frac{dy}{dx}(\frac{1}{2}(e^y+e^{-y}))=1\\
    \frac{dx}{dy}=(\frac{1}{2}(e^y+e^{-y}))\Rightarrow\\
    \frac{dx}{dy}=\cosh{y}\Rightarrow\frac{dy}{dx}=\frac{1}{\cosh{y}}\\
    \text{From the definition: }\sinh^2{x}-\cosh^2{x}=-1\\
    \cosh{y}=\sqrt{(\sinh{y})^2+1}\\
    \frac{dy}{dx}=\frac{1}{\cosh{y}}=\frac{1}{\sqrt{(\sinh{y})^2+1}}=\frac{1}{\sqrt{x^2+1}}
    $
    
    \item
 
        \(x^2+y^2=25 \)\\
        \(2x+2y\frac{dy}{dx}=0\)\\
        \(\frac{dy}{dx}=-\frac{x}{y} \)\\
        \(\frac{dy}{dx}|_{(3,4)}=-\frac{3}{4}\) \\
        \(\frac{dx}{dt}=\frac{dx}{dy}.\frac{dy}{dt}\)\\
        \( \frac{dx}{dt}=-\frac{4}{3}\times-2=\frac{8}{3}\)
\end{enumerate}
\end{spacing}
\end{document}