\documentclass[../main.tex]{subfiles}
\graphicspath{{\subfix{../images/}}}
\begin{document}
\hypertarget{quadraticsanswers}{\subsection*{Answers - Quadratics (\hyperlink{quadraticslink}{page \pageref{quadratics}})}}

\label{Quadratics answers}
\begin{spacing}{1.5}
\begin{enumerate}
    \item
    \((2^2)^x+2^x-24=0\)\\
    \((2^x)^2+2^x-24=0\)\\
    Making the substitution \(u=2^x\)\\
    \(u^2+2u-24=0\)\\
    \(u=4.42, -5.42\)\\
    \(2^x\) can never be negative so we can ignore the -5.42 solution.\\
    \(2^x=4.42\)\\
    \(\ln{2^x}=\ln{4.42}\)\\
    \(x\ln{2}=\ln{4.42}\)\\
    \(x=\frac{\ln{4.42}}{\ln{2}}\)\\
    \(x=2.14\) (1dp)
    \item 
    Rearrange to \(9^x-6^x-4^x=0\)\\
    We need a constant so divide through by the lowest term.\\
    \(
    \frac{9^x}{4^x}-\frac{6^x}{4^x}-\frac{4^x}{4^x}=0\\
    (\frac{9}{4})^x-(\frac{6}{4})^x-1=0\\
    ((\frac{3}{2})^2)^x-(\frac{3}{2})^x-1=0\\
    ((\frac{3}{2})^x)^2-(\frac{3}{2})^x-1=0\\ 
    \)
    Use the substitution \(u=(\frac{3}{2})^x\)\\
    \(
    u^2-u-1=0\\
    u-1.618, -0.618\\
    \)
    \((\frac{3}{2})^x\) can never be negative so we ignore -0.618.\\
    \(
    (\frac{3}{2})^x=1.618\\
    \ln{(\frac{3}{2})^x}=\ln{1.618}\\
    x\ln(\frac{3}{2})=\ln{1.6.18}\\
    x=\frac{\ln{1.618}}{\ln{\frac{3}{2}}}\\
    x=1.187
    \)
    \item 
    We need a constant so divide through by the lowest term.\\
    \(
    8(\frac{9^x}{4^x})+3(\frac{6^x}{4^x})-81=0\\
    8(\frac{9}{4})^x+3(\frac{6}{4})^x-81=0\\
    8((\frac{3}{2})^2)^x+3(\frac{3}{2})^x-81=0\\
    8((\frac{3}{2})^x)^2+3(\frac{3}{2})^x-81=0\\
    \)
    Use the substitution \(u=(\frac{3}{2})^x\)\\
    \(8u^2+3u-81=0\)\\
    \(u=3,-3.375\)\\
    Since \((\frac{3}{2})^x\) can never be negative, we can ignore the -3.375 solution.\\
    \((\frac{3}{2})^x=3\)\\
    \(\ln{(\frac{3}{2})^x}=\ln{3}\)\\
    \(x\ln{(\frac{3}{2})}=\ln{3}\)\\
    \(x=\frac{\ln{3}}{\ln{\frac{3}{2}}}\)=2.71
    \item 
    We need a constant so divide through by the lowest term.\\
    \(
    (\frac{25^x}{9^x})+2(\frac{15^x}{9^x})-24=0\\
    (\frac{25}{9})^x+2(\frac{15}{9})^x-24=0\\
    ((\frac{5}{3})^2)^x+2(\frac{5}{3})^x-24=0\\
    ((\frac{5}{3})^x)^2+2(\frac{5}{3})^x-24=0\\
    \)
    Use the substitution \(u=(\frac{5}{3})^x\)\\
    \(u^2+2u-24=0\)\\
    \(u=4,-6\)\\
    Since \((\frac{5}{3})^x\) can never be negative, we can ignore the -6 solution.\\
    \((\frac{5}{3})^x=4\)\\
    \(\ln{(\frac{5}{3})^x}=\ln{4}\)\\
    \(x\ln{(\frac{5}{3})}=\ln{4}\)\\
    \(x=\frac{\ln{4}}{\ln{\frac{5}{3}}}\)=2.714
\end{enumerate}


\end{spacing}
\end{document}