\documentclass[../main.tex]{subfiles}
\graphicspath{{\subfix{../images/}}}
\begin{document}

\hypertarget{camelprincipleanswers}{\subsection*{Answers - Camel principle (\hyperlink{camelprinciplelink}{page \pageref{Camel Principle}})}}

\label{Camel principle answers}
\begin{enumerate}
    \item
    \(\int \frac{x}{x+1}\,dx=\int \frac{x + 1 - 1}{x+1}\,dx\)

    \(= \int \frac{x+1}{x+1}\,dx - \int \frac{1}{x+1}\,dx\)

    \(= \int 1\,dx - \int \frac{1}{x+1}\,dx\)

    \(= x - \ln{|x+1|}+c\)

    \item 
    \(\int \frac{1}{1+e^x}\,dx=\int \frac{1+e^x-e^x}{1+e^x}\,dx\)
    
    \(= \int \frac{1+e^x}{1+e^x}\,dx-\int \frac{e^x}{1+e^x}\,dx\)

    \(= \int 1\,dx-\int \frac{e^x}{1+e^x}\,dx\)

    \(= x-\ln{|1+e^x|}+c\)
    
    \item
    \(\int \frac{2}{2 + e^{2x}}\,dx = \int \frac{2+e^{2x}-e^{2x}}{2+e^{2x}}\,dx\)
    
    \(= \int \frac{2+e^{2x}}{2+e^{2x}}\,dx - \int \frac{e^{2x}}{2+e^{2x}}\,dx\)

    Change the second integral into the form $\int \frac{f'(x)}{f(x)}\,dx$:

    \(= \int 1\,dx + \frac{1}{2}\int \frac{2e^{2x}}{2+e^{2x}}\,dx\) 

    \(= x + \frac{1}{2}\ln{|2+e^{2x}|}+c\)

    \item
    \(\int \frac{18x}{9x^2 -24x + 16}\,dx = \int \frac{18x - 24 + 24}{9x^2 - 24x + 16}\,dx\)

    \(= \int \frac{18x - 24}{9x^2-24x+16}\,dx + \int \frac{24}{9x^2-24x+16}\,dx\)

    \(= \ln{|9x^2-24x+16|} + \int \frac{24}{(3x-4)^2}\,dx\)

    To solve the second integral, use the substitution $u=3x-4$:

    $du = 3 dx \rightarrow \frac{1}{3}du = dx$

    Rewrite the second integral in terms of $u$:

    \(= \ln{|9x^2-24x+16|} + \int \frac{8}{u^2}\,du\)

    \(= \ln{|9x^2-24x+16|} + 8\int u^{-2}\,du\)

    \(= \ln{|9x^2-24x+16|} - \frac{8}{u} + c\)

    \(= \ln{|9x^2-24x+16|} - \frac{8}{3x-4} + c\)

    \item 
    \(\int \frac{1}{1+\sqrt{e^x}}\,dx=\int \frac{1+\sqrt{e^x}-\sqrt{e^x}}{1+\sqrt{e^x}}\,dx\)

    \(=\int \frac{1+\sqrt{e^x}}{1+\sqrt{e^x}}\,dx-\int \frac{\sqrt{e^x}}{1+\sqrt{e^x}}\,dx\)

    \(=\int 1\,dx-\int \frac{\sqrt{e^x}}{1+\sqrt{e^x}}\,dx\)

    \(x-\int \frac{\sqrt{e^x}}{1+\sqrt{e^x}}\,dx\)

    For the remaining integral, use the substitution\(u=\sqrt{e^x}\), meaning that \(u^2=e^x\).

    \(x=\ln{u^2}=2\ln{u}\)

    \(dx=\frac{2}{u}\,du\)

    \(x-\int \frac{u}{1+u}\frac{2\,du}{u}=x-2\int \frac{1}{1+u}\,du\)

    \(x-2\ln{|1+u|}+c\)

    \(x-2\ln{|1+\sqrt{e^x}|}+c\)
    
    \item
    \(7\int \frac{x}{4x^2+20x+25}\,dx\)

    We know the denominator differentiates to $8x+20$ so first we will change the numerator to $8x$ by using the Camel Principle multiplicatively:

    \(\frac{7}{8}\int \frac{8x}{4x^2+20x+25}\,dx\)

    Next, we use it additively to get the 20 we need in the numerator:

    \(\frac{7}{8}\int \frac{8x + 20 - 20}{4x^2+20x+25}\,dx= \frac{7}{8}\int \frac{8x + 20}{4x^2+20x+25}\,dx-\frac{7}{8}\int \frac{20}{4x^2+20x+25}\,dx\)

    \(=\frac{7}{8}\ln{|4x^2+20x+25} - \frac{7}{8}\int \frac{20}{4x^2+20x+25}\,dx\)

    The denominator of the second integral factorises to $(2x+5)^2$, so we can use the substitution $u=2x+5$

    $du = 2\,dx \rightarrow \frac{1}{2}du=dx$

    \(=\frac{7}{8}\ln{|4x^2+20x+25|} - \frac{7}{8}.\frac{1}{2}\int \frac{20}{u^2}\,du\)

    \(=\frac{7}{8}\ln{|4x^2+20x+25|} - \frac{7}{16}\int \frac{20}{u^2}\,du\)

    \(=\frac{7}{8}\ln{|4x^2+20x+25|} - \frac{140}{16}\int u^{-2}\,du\)

    \(=\frac{7}{8}\ln{|4x^2+20x+25|} + \frac{35}{4u}+c\)

    \(=\frac{7}{8}\ln{|4x^2+20x+25|} + \frac{35}{8x+20}+c\)

    \item 
    \(\int \sec{x}\,dx\)

    In this case we will use the Camel Principle multiplicatively, multiplying by \(\frac{\sec{x}+\tan{x}}{\sec{x}+\tan{x}}\)

    This gives us the integral:

    \(\int \frac{\sec^2{x}+\sec{x}\tan{x}}{\sec{x}+\tan{x}}\,dx\)

    This is in the format \(\frac{f'(x)}{f(x)}\), which integrates to \(\ln{|f(x)|}+c\)

    Therefore, our integral is \(\ln{|\sec{x}+\tan{x}|}+c\)

    \item 
    \(\int \csc{\theta}\,d\theta\)

    To integrate, first multiply by \(\frac{\csc{\theta}-\cot{\theta}}{\csc{\theta}+\cot{\theta}}\)

    This changes the integral to:

    \(\int \frac{\csc^2{\theta}-\csc{\theta}\cot{\theta}}{\csc{\theta}-\cot{\theta}}\)

    This is in the form \(\frac{f'(x)}{f(x)}\), therefore the integral is \(\ln{|\csc{\theta}-\tan{\theta}|}+c\)
    
    \item 
    $\int \frac{1}{1+\tan{x}}\, dx$

    Change the $\tan{x}$ into $\frac{\sin{x}}{\cos{x}}$ and simplify:

    $\int \frac{1}{1+\frac{\sin{x}}{\cos{x}}}\,dx$

    $\int \frac{1}{\frac{\cos{x}+\sin{x}}{\cos{x}}}\,dx$

    $\int \frac{\cos{x}}{\sin{x}+\cos{x}}\,dx$

    Now we can use the Camel Principle. First, we double the fraction:

    $\frac{1}{2}\int \frac{2\cos{x}}{\sin{x}+\cos{x}}\,dx$

    Then we add and subtract $\sin{x}$ from the numerator:

    $\frac{1}{2}\int \frac{2\cos{x}+\sin{x}-\sin{x}}{\sin{x}+\cos{x}}\,dx$

    Separate into two fractions:

    $\frac{1}{2}\int \Bigl(\frac{\cos{x}+\sin{x}}{\sin{x}+\cos{x}}+\frac{\cos{x}-\sin{x}}{\sin{x}+\cos{x}}\Bigr)\,dx$

    Split into two integrals and simplify:

    $\frac{1}{2}\int 1\,dx+\frac{1}{2}\int \frac{\cos{x}-\sin{x}}{\sin{x}+\cos{x}}\,dx$

    The first fraction integrates easily. The second integral is in the form $\int \frac{f'(x)}{f(x)}\, dx$, therefore:

    $\frac{x}{2}+\frac{1}{2}\ln{|\sin{x}+\cos{x}|}+c$

\end{enumerate}

\end{document}