\documentclass[../main.tex]{subfiles}
\graphicspath{{\subfix{../images/}}}
\begin{document}


\subsection*{Answers - Trigonometric identities (page \pageref{Trig identities})}
\label{Trig identities answers}.

For each of the following, show that:
\begin{enumerate}
    \item LHS = $\frac{\sin{A}+\cos{A}}{\sin{A}-\cos{A}}\times \frac{\sin{A}+\cos{A}}{\sin{A}+\cos{A}}$

    $\frac{\sin^2{A}+2\sin{A}\cos{A}+\cos^2{A}}{\sin^2{A}-\cos^2{A}}$

    Using the $\sin^2{A}+\cos^2{A}=1$ and the $\cos{2A}$ identities:

    $\frac{1+2\sin{A}\cos{A}}{1-2\cos^2{A}}$
    
    = RHS as required

    \item LHS = $\frac{\sin{2A}}{1+\cos{2A}}$

    Using cosine double angle rule:

    $ = \frac{\sin{2A}}{1+2\cos^2{A}-1}$

    $ = \frac{2\sin{A}\cos{A}}{2\cos^2{A}}$

    $ = \frac{\sin{A}}{\cos{A}}$

    $ = \tan{A}$ as required

    
    \item LHS = $2\sin{A}\cos{A}$

    RHS = $\frac{\frac{2\sin{A}}{\cos{A}}}{1+\frac{\sin^2{A}}{\cos^2{A}}}$

    = $\frac{\frac{2\sin{A}}{\cos{A}}}{1+\frac{\sin^2{A}}{\cos^2{A}}}\times \frac{\cos^2{A}}{\cos^2{A}}$

    = $\frac{2\sin{A}\cos{A}}{\cos^2{A}+\sin^2{A}}$

    = $2\sin{A}\cos{A}$
    
    LHS = RHS as required

    \item $\frac{\sin{2A}}{\sin{A}}-\frac{\cos{2A}}{\cos{A}}=\sec{A}$
    
    LHS = $\frac{2\sin{A}\cos{A}}{\sin{A}}-\frac{2\cos^2{A}-1}{\cos{A}}$

    = $2\cos{A}-2\cos{A}+\frac{1}{\cos{A}}$

    = $\sec{A}$
    
    = RHS as required
    
    \item 
    
    LHS = $\sec^2{A}-2\sec{A}\tan{A}+\tan^2{A}$

    $= \frac{1}{\cos^2{A}}-\frac{2\sin{A}}{\cos^2{A}}+\frac{\sin^2{A}}{\cos^2{A}}$

    $= \frac{(1-\sin{A})^2}{1-\sin^2{A}}$

    $= \frac{(1-\sin{A})^2}{(1-\sin{A})(1+\sin{A})}$

    $= \frac{1-\sin{A}}{1+\sin{A}}$
    
    = RHS as required

    \item RHS = $\sqrt{\frac{1-(1-2\sin^2{A})}{1+(2\cos^2{A}-1)}}$

    = $\sqrt{\frac{2\sin^2{A}}{2\cos^2{A}}}$

    = $\sqrt{\frac{\sin^2{A}}{\cos^2{A}}}$

    = $\frac{\sin{A}}{\cos{A}}$

    = $\tan{A}$

    = LHS as required

    \item LHS = $\frac{\csc^2{A}-1}{\cos^2{A}}+\frac{1}{1-\sin^2{A}}$

    = $\frac{\csc^2{A}}{\cos^2{A}}$

    = $\sec^2{A}\csc^2{A}$

    = RHS as required

    \item LHS = $\frac{\cos{A}}{1+\sin{A}}$

    = $\frac{\cos{A}}{1+\sin{A}} \times \frac{1-\sin{A}}{1-\sin{A}}$

    = $\frac{\cos{A}(1-\sin{A})}{1-\sin^2{A}}$

    = $\frac{\cos{A}(1-\sin{A})}{\cos^2{A}}$

    = $\frac{1-\sin{A}}{\cos{A}}$

    = RHS as required

    \item Rewriting LHS:

    LHS = $\frac{2}{\sin{4A}}+\frac{2\cos{4A}}{\sin{4A}}$

    = $\frac{2(1+\cos{4A})}{\sin{4A}}$

    Using the sine and the cosine double-angle rules:

    = $\frac{2(2\cos^2{2A})}{2\sin{2A}\cos{2A}}$

    = $\frac{2\cos{2A}}{\sin{2A}}$

    Using double-angle rules again:

    = $\frac{2(\cos^2{A}-\sin^2{A})}{2\sin{A}\cos{A}}$

    = $\frac{\cos^2{A}-\sin^2{A}}{\sin{A}\cos{A}}$

    = $\frac{\cos^2{A}}{\sin{A}\cos{A}}-\frac{\sin^2{A}}{\sin{A}\cos{A}}$

    = $\cot{A}-\tan{A}$

    = RHS as required

    \item LHS = $\frac{\sin{(2A+A)}}{2\sin{A}\cos{A}-\sin{A}}$

    = $\frac{\sin{2A}\cos{A}+\cos{2A}\sin{A}}{2\sin{A}\cos{A}-\sin{A}}$

    = $\frac{2\sin{A}\cos^2{A}+\cos{2A}\sin{A}}{2\sin{A}\cos{A}-\sin{A}}$

    = $\frac{2\cos^2{A}+\cos{2A}}{2\cos{A}-1}$

    = $\frac{2\cos^2{A}+2\cos^2{A}-1}{2\cos{A}-1}$

    = $\frac{4\cos^2{A}-1}{2\cos{A}-1}$

    = $\frac{(2\cos{A}+1)(2\cos{A}-1)}{2\cos{A}-1}$

    = $2\cos{A}+1$

    = RHS as required

    \item LHS = $\frac{1+\cos{A}}{1-\cos{A}}$

    = $\frac{1+\cos{A}}{1-\cos{A}}\times \frac{1+\cos{A}}{1+\cos{A}}$

    = $\frac{(1+\cos{A})^2}{1-\cos^2{A}}$

    = $\frac{(1+\cos{A})^2}{\sin^2{A}}$

    = $\Bigl(\frac{1+\cos{A}}{\sin{A}}\Bigr)^2$

    = $\Bigl(\frac{1}{\sin{A}}+\frac{\cos{A}}{\sin{A}}\Bigr)^2$

    = $(\csc{A}+\cot{A})^2$

    = RHS as required

    \item RHS = $\frac{1-\tan^2{A}}{1+\tan^2{A}}$

    = $\frac{\frac{\cos^2{A}-\sin^2{A}}{\cos^2{A}}}{\frac{\cos^2{A}+\sin^2{A}}{\cos^2{A}}}$

    = $\frac{\cos^2{A}-\sin^2{A}}{\cos^2{A}+\sin^2{A}}$

    = $\cos^2{A}-\sin^2{A}$

    = $\cos{2A}$

    = LHS as required

    \item $\cos{3A}=4\cos^3{A}-3\cos{A}$
    
    LHS = $\cos{3A}$

    = $\cos{(2A+A)}$

    = $\cos{2A}\cos{A}-\sin{2A}\sin{A}$

    = $(2\cos^2{A}-1)\cos{A}-2\sin^2{A}\cos{A}$

    = $2\cos^3{A}-\cos{A}-2(1-\cos^2{A})\cos{A}$

    = $2\cos^3{A}-\cos{A}-2\cos{A}+2\cos^3{A}$

    = $4\cos^3{A}-3\cos{A}$

    = RHS as required

    \item $\cos{4A}=1-8\sin^2{A}\cos^2{A}$
    
    LHS = $\cos{(2A+2A)}$

    = $\cos{2A}\cos{2A}-\sin{2A}\sin{2A}$

    = $(2\cos^2{A}-1)(1-2\sin^2{A})-4\sin^2{A}\cos^2{A}$

    = $2\cos^2{A}-4\sin^2{A}\cos^2{A}-1+2\sin^2{A}-4\sin^2{A}\cos^2{A}$

    = $2(\sin^2{A}+\cos^2{A})-1-8\sin^2{A}\cos^2{A}$

    = $1-8\sin^2{A}\cos^2{A}$

    = RHS as required

    \item $\tan{3A}=\frac{3\tan{A}-\tan^3{A}}{1-3\tan^2{A}}$
    
    LHS = $\tan{(2A+A)}$

    = $\frac{\tan{2A}+\tan{A}}{1-\tan{2A}\tan{A}}$

    = $\frac{\frac{2\tan{A}}{1-\tan^2{A}}+\tan{A}}{1-\frac{2\tan{A}}{1-\tan^2{A}}\tan{A}}$

    = $\frac{\frac{2\tan{A}+\tan{A}(1-\tan^2{A})}{1-\tan^2{A}}}{\frac{1-\tan^2{A}-2\tan^2{A}}{1-\tan^2{A}}}$

    = $\frac{3\tan{A}-\tan^3{A}}{1-3\tan^2{A}}$

    = RHS as required

    \item $\tan{4A}=\frac{4\tan{A}-4\tan^3{A}}{1-6\tan^2{A}+\tan^4{A}}$
    
    LHS = $\tan{(2A+2A)}$

    = $\frac{\tan{2A}+\tan{2A}}{1-\tan{2A}\tan{2A}}$

    = $\frac{2\tan{2A}}{1-\tan^2{2A}}$

    = $\frac{2\Bigl(\frac{2\tan{A}}{1-\tan^2{A}}\Bigr)}{1-\Bigl(\frac{2\tan{A}}{1-\tan^2{A}}\Bigr)^2}$

    = $\frac{\frac{4\tan{A}}{1-\tan^2{A}}}{\frac{(1-\tan^2{A})^2-4\tan^2{A}}{(1-\tan^2{A})^2}}$

    = $\frac{\frac{4\tan{A}}{1-\tan^2{A}}}{\frac{1-6\tan^2{A}+\tan^4{A}}{(1-\tan^2{A})^2}}$

    = $\frac{4\tan{A}(1-\tan^2{A})^2}{(1-\tan^2{A})(1-6\tan^2{A}+\tan^4{A})}$

    = $\frac{4\tan{A}-4\tan^3{A}}{1-6\tan^2{A}+\tan^4{A}}$

    = RHS as required

    \item $4\sin^3{A}\cos{3A}+4\cos^3{A}\sin{3A}=3\sin{4A}$

    LHS = $2\sin^2{A}(2\sin{A}\cos{3A})+2\cos^2{A}(2\cos{A}\sin{3A})$

    Using product identities:

    = $2\sin^2{A}(\sin{4A}-\sin{2A})+2\cos^2{A}(\sin{4A}+\sin{2A})$

    = $2\sin^2{A}\sin{4A}-2\sin^2{A}\sin{2A}+2\cos^2{A}\sin{4A}+2\cos^2{A}\sin{2A}$

    = $2\sin{4A}(\sin^2{A}+\cos^2{A})+2\sin{2A}(\cos^2{A}-\sin^2{A})$

    = $2\sin{4A}+2\sin{2A}\cos{2A}$

    Using sine double angle rule

    = $2\sin{4A}+\sin{4A}$

    = $3\sin{4A}$

    = RHS as required


\end{enumerate}
Harder problems (including old scholarship questions):
\begin{enumerate}
    \setcounter{enumi}{18}
    \item $\frac{\csc{A}-\cot{A}}{\csc{A}+\cot{A}}+\frac{\csc{A}+\cot{A}}{\csc{A}-\cot{A}}\equiv 2+4\cot^2{A}$
    
    LHS = $\frac{(\csc{A}-\cot{A})^2+(\csc{A}+\cot{A})^2}{\csc^2{A}-\cot^2{A}}$

    From the identity $\cot^2{A}+1=\csc^2{A}$:

    = $(\csc{A}-\cot{A})^2+(\csc{A}+\cot{A})^2$

    = $\csc^2{A}-2\csc{A}\cot{A}+\cot^2{A}+\csc^2{A}+2\csc{A}\cot{A}+\cot^2{A}$

    = $2\csc^2{A}+2\cot^2{A}$

    = $2(\cot^2{A}+1)+2\cot^2{A}$

    = $2 + 4\cot^2{A}$

    = RHS as required

    \item $\frac{1-\sin{A}}{1-\sec{A}}-\frac{1+\sin{A}}{1+\sec{A}}\equiv 2\cot{A}(\cos{A}-\csc{A})$
    
    LHS = $\frac{(1-\sin{A})(1|\sec{A})-(1+\sin{A})(1+\sec{A})}{1-\sec^2{A}}$

    = $\frac{2\sec{A}-2\sin{A}}{-\tan^2{A}}$

    = $\frac{2\sin{A}}{\tan^2{A}}-\frac{2\sec{A}}{\tan^2{A}}$

    = $\frac{2\sin{A}}{\frac{\sin^2{A}}{\cos^2{A}}}-\frac{2\sec{A}}{\frac{\sin^2{A}}{\cos^2{A}}}$

    = $\frac{2\cos^2{A}}{\sin{A}}-\frac{2\cos{A}}{\sin^2{A}}$

    = $2\frac{\cos{A}}{\sin{A}}\cos{A}-2\frac{\cos{A}}{\sin{A}}\frac{1}{\sin{A}}$

    = $2\cot{A}\cos{A}-2\cot{A}\csc{A}$

    = $2\cot{A}(\cos{A}-\csc{A})$

    = RHS as required

    \item $\frac{1+\cos{A}}{1-\cos{A}}\equiv (\csc{A}+\cot{A})^2$
    
    LHS = $\frac{(1+\cos{A})^2}{1-\cos^2{A}}$

    = $\frac{1+2\cos{A}+\cos^2{A}}{\sin^2{A}}$

    = $\frac{1}{\sin^2{A}}+\frac{2\cos{A}}{\sin^2{A}}+\frac{\cos^2{A}}{\sin^2{A}}$

    = $\csc^2{A}+2\frac{\cos{A}}{\sin{A}}\frac{1}{\sin{A}}+\cot^2{A}$

    = $\csc^2{A}+2\csc{A}\cot{A}+\cot^2{A}$

    = $(\csc{A}+\cot{A})^2$

    = RHS as required

    \item $\frac{\sin{(\pi-B)}-\sin{A}}{\cos{A}+\cos{(\pi - B)}}\equiv \frac{\cos{A}+\cos{B}}{\sin{B}+\sin{(\pi - A)}}$
    
    For this, manipulate both sides and make them equal to each other.

    LHS = $\frac{\sin{\pi}\cos{B}-\cos{\pi}\sin{B}-\sin{A}}{\cos{A}+\cos{\pi}\cos{B}+\sin{\pi}\sin{B}}$

    = $\frac{\sin{B}-\sin{A}}{\cos{A}-\cos{B}}$

    RHS = $\frac{\cos{A}+\cos{B}}{\sin{B}+\sin{\pi}\cos{A}-\sin{A}\cos{\pi}}$

    = $\frac{\cos{A}+\cos{B}}{\sin{B}+\sin{A}}$

    Equating:

    $\frac{\sin{B}-\sin{A}}{\cos{A}-\cos{B}}=\frac{\cos{A}+\cos{B}}{\sin{B}+\sin{A}}$

    = $\sin^2{B}-\sin^2{A}=\cos^2{A}-\cos^2{B}$

    = $\sin^2{B}+\cos^2{B}=\sin^2{A}+\cos^2{A}$

    = $1 = 1$

    True statement, therefore the original statement is also true.

    \item $\frac{\csc{A}-\sec{A}}{\csc{A}+\sec{A}}(\cot{A}-\tan{A})\equiv \sec{A}\csc{A}-2$
    
    \item $(\sec{A}-2\sin{A})(\csc{A}+2\cos{A})\sin{A}\cos{A}\equiv (\cos^2{A}-\sin^2{A})^2$
    
    LHS = $\cos{A}(\sec{A}-2\sin{A})\sin{A}(\csc{A}+2\cos{A})$

    = $(1-2\sin{A}\cos{A})(1+2\sin{A}\cos{A})$

    = $(1-\sin{2A})(1+\sin{2A})$

    = $1-\sin^2{2A}$

    = $\cos^2{2A}$

    = $(\cos^2{A}-\sin^2{A})^2$

    = RHS as required

    \item 2018 Scholarship exam:
    
    $\frac{\cos{\theta}}{1+\sin{\theta}}-\frac{\sin{\theta}}{1+\cos{\theta}}=\frac{2(\cos{\theta}-\sin{\theta})}{1+\sin{\theta}+\cos{\theta}}$

    LHS = $\frac{\cos{\theta}(1+\cos{\theta})-\sin{\theta}(1+\sin{\theta})}{(1+\sin{\theta})(1+\cos{\theta})}$

    = $\frac{\cos{\theta}+\cos^2{\theta}-\sin{\theta}-\sin^2{\theta}}{1+\sin{\theta}+\cos{\theta}+\sin{\theta}\cos{\theta}}$

    = $\frac{\cos{\theta}-\sin{\theta}+\cos^2{\theta}-\sin^2{\theta}}{1+\sin{\theta}+\cos{\theta}+\sin{\theta}\cos{\theta}}$

    = $\frac{\cos{\theta}-\sin{\theta}+(\cos{\theta}-\sin{\theta})(\cos{\theta}+\sin{\theta})}{1+\sin{\theta}+\cos{\theta}+\sin{\theta}\cos{\theta}}$

    Factorising the numerator:

    = $\frac{(\cos{\theta}-\sin{\theta})(1+\cos{\theta}+\sin{\theta})}{1+\sin{\theta}+\cos{\theta}+\sin{\theta}\cos{\theta}}$ 

    Double everything:

    = $\frac{2(\cos{\theta}-\sin{\theta})(1+\cos{\theta}+\sin{\theta})}{2+2\sin{\theta}+2\cos{\theta}+2\sin{\theta}\cos{\theta}}$

    = $\frac{2(\cos{\theta}-\sin{\theta})(1+\cos{\theta}+\sin{\theta})}{1+\sin^2{\theta}+\cos^2{\theta}+2\sin{\theta}+2\cos{\theta}+2\sin{\theta}\cos{\theta}}$

    = $\frac{2(\cos{\theta}-\sin{\theta})(1+\sin{\theta}+\cos{\theta})}{(1+\sin{\theta}+\cos{\theta})^2}$

    = $\frac{2(\cos{\theta}-\sin{\theta})}{1+\sin{\theta}+\cos{\theta}}$

    = RHS as required

    \item 2017 Scholarship exam:
    
    $\cos{(5\theta)}=16\cos^5{\theta}-20\cos^3{\theta}+5\cos{\theta}$

    LHS = $\cos{(4\theta + \theta)}$

    = $\cos{4\theta}\cos{\theta}-\sin{4\theta}\sin{\theta}$

    Use double angle rules where the double angle is $4\theta$ so the angle is $2\theta$

    = $(2\cos^2{2\theta}-1)\cos{\theta}-2\sin{2\theta}\cos{2\theta}\sin{\theta}$

    Use double-angle rules for cosine and sine:

    = $\Bigl(2(2\cos^2{\theta}-1)^2 -1\Bigr)\cos{\theta}-4\sin^2{\theta}\cos{\theta}\cos{2\theta}$

    = $(8\cos^4{\theta}-8\cos^2{\theta}+1)\cos{\theta}-4(1-\cos^2{\theta})\cos{\theta}\cos{2\theta}$

    = $8\cos^5{\theta}-8\cos^3{\theta}+\cos{\theta}+4(\cos^3{\theta}-\cos{\theta})(2\cos^2{\theta}-1)$

    = $8\cos^5{\theta}-8\cos^3{\theta}+\cos{\theta}+8\cos^5{\theta}-12\cos^3{\theta}+4\cos{\theta}$

    = $16\cos^5{\theta}-20\cos^3{\theta}+5\cos{\theta}$

    = RHS as required

    
\end{enumerate}





\end{document}