\documentclass[../main.tex]{subfiles}
\graphicspath{{\subfix{../images/}}}
\begin{document}

\subsection*{Answers - Log problems (page \pageref{Log problems})}
\label{Log problems answers}
\begin{enumerate}[itemsep=0.4cm]
    \item     
    By taking $\log_3$ of both sides we can form a quadratic:

    \(\log_3(x^{\log_3(x)})=\log_3(81x^3)\)

    \(\log_3(x)\times \log_3(x)=\log_3(81)+\log_3(x^3)\)

    \((\log_3(x))^2=4+3\log_3(x)\)

    Using the substitution $u=\log_3(x)$:

    \(u^2-3u-4=0\)

    \(u=-1,4\)

    Solving:

    \(\log_3(x)=-1 \rightarrow x=3^{-1} = \frac{1}{3}\)

    \(\log_3(x)=4 \rightarrow x=3^4 = 81\)

    \item 
    \(4^{x-1}=2^x +48\)

    \((2^2)^{x-1}=2^x +48\)

    \(2^{2x-2}=2^x +48\)

    \(\frac{2^{2x}}{2^2}=2^x +48\)

    \(\frac{(2^x)^2}{4}=2^x +48\)

    Substitute $u=2^x$ and solve the quadratic:

    \(\frac{u^2}{4}-u-48=0\)

    \(u=16, -12\)

    Reverse substitution:

    \(2^x=16 \rightarrow x=4\)

    \(2^x = -12 \rightarrow\) Not possible

    Therefore the only solution is $x=4$

    \item Use the change of base formula to change to base 10:

    \(\frac{\log(y)}{\log(x)}+\frac{\log(x)}{\log(y)}=2\)

    \(\frac{(\log(y))^2 + (\log(x))^2}{\log(x)\log(y)}=2\)

    \((\log(y))^2 + (\log(x))^2=2\log(x)\log(y)\)

    \((\log(y))^2 -2\log(x)\log(y) + (\log(x))^2=0\)

    This is a perfect square, so factorise:

    \((\log(x)-\log(y))^2=0\)

    \(\log(x)=\log(y)\)

    \(x=y\)

    \(\frac{x}{y}+\frac{y}{x}=\frac{x}{x}+\frac{x}{x}=2\)

    \item 
    If $\sqrt{\log_a(b)}+\sqrt{\log_b(a)}=2$, then find the value of $\log_{ab}(a)-\log_{\frac{1}{ab}}(b)$

    Squaring the equation gives us:

    \(\log_a(b)+2\sqrt{\log_a(b)\log_b(a)}+\log_b(a)=4\)

    Use change of base formula to simplify:

    \(\frac{\log(b)}{\log(a)}+2\sqrt{\frac{\log(b)}{\log(a)}\times \frac{\log(a)}{\log(b)}}+\frac{\log(a)}{\log(b)}=4 \)

    \(\frac{\log(b)}{\log(a)}+2\sqrt{1}+\frac{\log(a)}{\log(b)}=4 \)

    \(\frac{\log(b)}{\log(a)}+2+\frac{\log(a)}{\log(b)}=4 \)

    \(\frac{\log(b)}{\log(a)}+\frac{\log(a)}{\log(b)}=2 \)

    \(\frac{(\log(b))^2+(\log(a))^2}{\log(a)\log(b)} =2\)

    \((\log(b))^2+(\log(a))^2=2\log(a)\log(b)\)

    \((\log(b))^2-2\log(a)\log(b+(\log(a))^2=)\)

    Perfect square:

    \((\log(b)-\log(a))^2=0 \)

    \(\log(a)=\log(b)\)

    \(a=b\)

    Substituting into $\log_{ab}(a)-\log_{\frac{1}{ab}}(b)$ we get $\log_{a^2}(a)-\log_{\frac{1}{a^2}}(a)$

    $\log_{a^2}(a)=\frac{1}{2}$ and $\log_{\frac{1}{a^2}}(a)=\frac{-1}{2}$

    \(\frac{1}{2}-\frac{-1}{2}=1\)


    \item 
    If $2^{3x-5}=3^{x+3}$ and $x=\log(864^{\log_{10}(y)})$, then find the value of $y^{\log_{10}\frac{8}{3}}$

    Taking log base 10 of both sides:

    \((3x-5)\log_{10}(2)=(x+3)\log_{10}(3)\)

    \(3x\log_{10}(2)-5\log_{10}(2)=x\log_{10}(3)+3\log_{10}(3)\)

    \(3x\log_{10}(2)-x\log_{10}(3)=5\log_{10}(2)+3\log_{10}(3)\)

    \(x(3\log_{10}(2)-\log_{10}(3))=5\log_{10}(2)+3\log_{10}(3)\)

    \(x=\frac{5\log_{10}(2)+3\log_{10}(3)}{3\log_{10}(2)-\log_{10}(3)}\)

    Simplify using log rules:

    \(x=\frac{\log_{10}(32)+\log_{10}(27)}{\log_{10}(8)-\log_{10}(3)}\)

    \(x=\frac{\log_{10}(864)}{\log_{10}(\frac{8}{3})}\)

    \(x=\frac{1}{\log_{10}(\frac{8}{3})}\times \log_{10}(864)\)

    \(x=\log_{10}(864)^{\frac{1}{\log_{10}(\frac{8}{3})}}\)

    Going back to the original question, this means that $\log_{10}(y)=\frac{1}{\log_{10}(\frac{8}{3})}$

    \(\log_{10}(\frac{8}{3})\log_{10}(y)=1\)

    \(\log_{10}(y)^{\log_{10}(\frac{8}{3})} = 1\)

    \(y^{\log_{10}(\frac{8}{3})}=10\)



    \item 
    \(7^0=\log_9(x^2+\sqrt{x+1}+8)\)

    \(1=\log_9(x^2+\sqrt{x+1}+8)\)

    \(9^1=x^2+\sqrt{x+1}+8 \)

    \(\sqrt{x+1}=1-x^2\)

    Squaring the equation:

    \(x+1=1-2x^2+x^4\)

    \(x^4-2x^2-x=0\)

    Solving, we get $x=0, -1, \frac{1\pm\sqrt{5}}{2}$

    Substituting back into the original equation (as we should because by squaring the equation we may have introduced false solutions), we find that $x=\frac{1\pm \sqrt{5}}{2}$ is not valid, therefore $x=0,-1$

    \item 
    If $\log_{16}(x)+\log_8(y)=11$ and $\log_8(x)+\log_{16}(y)=10$ then find the value of $\frac{y}{x^2}$

    Because bases are all powers of 2, we will use the change of base formula to make the new base 2.

    Equation 1: $\frac{\log_2(x)}{\log_2(16)}+\frac{\log_2(y)}{\log_2(8)}=11 $

    Becomes $\frac{\log_2(x)}{4}+\frac{\log_2(y)}{3}=11 $ which we can rearrange into $3\log_2(x)+4\log_2(y)=132$

    Equation 2: $\frac{\log_2(x)}{\log_2(8)}+\frac{\log_2(y)}{\log_2(16)}=10$

    Becomes $\frac{\log_2(x)}{3}+\frac{\log_2(y)}{4}=10$ which we can rearrange into $3\log_2(x)+3\log_2(y)=120$

    Solving simultaneously:

    \(3\log_2(x)+4\log_2(y)=132\)

    \(3\log_2(x)+3\log_2(y)=120\)

    \(\log_2(y)=24\)

    \(y=2^{24}\)

    Solve for x by substituting back into equation 1:

    \(3\log_2(x)+4\log_2(2^{24})=132\)

    \(3\log_2(x)+4\times 24=132\)

    \(3\log_2(x)=36\)

    \(log_2(x)=12\)

    \(x=2^{12}\)

    To find the value of $\frac{y}{x^2}$ we substitute:

    \(\frac{y}{x^2}=\frac{2^{24}}{(2^{12})^2}=\frac{2^{24}}{2^{24}}=1\)

    \item 
    Use the change of base formula to change the base to 2:

    \(\frac{\log_2(4)}{\log_2(\log_2(x))}=\log_2\Bigl(\frac{\log_2(x)}{\log_2(4)}\Bigr) \)

    \(\frac{2}{\log_2(\log_2(x))}=\log_2\Bigl(\frac{\log_2(x)}{2}\Bigr) \)

    \(\frac{2}{\log_2(\log_2(x))}=\log_2(\log_2(x))-\log_2(2) \)

    \(\frac{2}{\log_2(\log_2(x))}=\log_2(\log_2(x))-1 \)

    \(2=(\log_2(x))^2-\log_2(\log_2(x))\)

    We have a quadratic in terms of $\log_2(\log_2(x))$, so we make a substitution:

    \(u=\log_2(\log_2(x))\)

    \(2=u^2-u\)

    \(u^2-u-2\)

    \(u=2, -1\)

    Reversing the substitution:

    \(\log_2(\log_2(x))=2\)

    \(\log_2(x)=2^2=4\)

    \(2^4=x \rightarrow x=16\)

    \(\log_2(\log_2(x))=-1\)

    \(\log_2(x)=2^{-1}=\frac{1}{2}\)

    \(2^{\frac{1}{2}}=x \rightarrow x=\sqrt{2}\)

    \(x=\sqrt{2}, 16\)

    \item 
    Use the change of base formula for each equation, then simplify (notice we are using bases that help us get whole number bases).

    Equation 1: \(\frac{\log_2(x)}{\log_2(4)}+\frac{\log_3(y)}{\log_3(9)}=2\)

    \(\frac{\log_2(x)}{2}+\frac{\log_3(y)}{2}=2\)

    \(\log_2(x)+\log_3(y)=4\)

    Equation 2: $\frac{\log_2(2)}{\log_2(x)}+\frac{\log_3(3)}{\log_3(y)}=1$

    $\frac{1}{\log_2(x)}+\frac{1}{\log_3(y)}=1$

    $\frac{\log_2(x)+\log_3(y)}{\log_2(x)\log_3(y)}=1$

    $\log_2(x)+\log_3(y)=\log_2(x)\log_3(y)$

    Substitute equation 1 into equation 2:

    $4=\log_2(x)\log_3(y)$

    Rearrange and make $\log_3(y)$ the subject:

    $\log_3(y)=\frac{4}{\log_2(x)}$

    Substitute into equation 1:

    $\log_2(x)+\frac{4}{\log_2(x)}=4$

    This is a quadratic in terms of $\log_2(x)$, so we substitute $u=\log_2(x)$:

    $u+\frac{4}{u}=4$

    $u^2-4u+4=0$

    $u=2$

    Reverse the substitution:

    $\log_2(x)=2$

    $x=2^2=4$

    Substitute into $\log_3(y)=\frac{4}{\log_2(x)}$

    $\log_3(y)=\frac{4}{\log_2(4)}$

    $\log_3(y)=2$

    $y=3^2=9$

    \item 
    If $\log_5(4), \log_5(2^x+\frac{1}{2})$ and $\log_5(2^x-\frac{1}{4})$ are in arithmetic progression, find the value of $x$ and also find the common difference.

    $\log_5(2^x+\frac{1}{2})-\log_5(4)=\log_5(2^x-\frac{1}{4})-\log_5(2^x+\frac{1}{2})$

    $2\log_5(2^x+\frac{1}{2})=\log_5(4)+\log_5(2^x-\frac{1}{4})$

    $2\log_5(2^x+\frac{1}{2})=\log_5 4(2^x-\frac{1}{4})$

    $2\log_5(2^x+\frac{1}{2})=\log_5 (4\times 2^x-1)$

    $\log_5(2^x+\frac{1}{2})^2=\log_5 (4\times 2^x-1)$

    $\log_5\Bigl(2^x+\frac{1}{2}\Bigr)^2-\log_5 (4\times 2^x-1)=0$

    $\log_5\Bigl(\frac{(2^x+\frac{1}{2})^2}{4\times 2^x -1}\Bigr)=0$

    $\frac{(2^x+\frac{1}{2})^2}{4\times 2^x -1}=1$

    $\Bigl(2^x+\frac{1}{2}\Bigr)^2=4\times 2^x -1$

    $(2^x)^2+2^x +\frac{1}{4}=4\times 2^x -1$

    $(2^x)^2 - 3\times 2^x +\frac{5}{4}=0$

    Substitute $u=2^x$:

    $u^2-3u+\frac{5}{4}=0$

    $u=\frac{5}{2},\frac{1}{2}$

    Reverse substitution:

    $2^x=\frac{1}{2} \rightarrow x=-1$

    $2^x=\frac{5}{2}$

    $x=\log_2{\frac{5}{2}}=\log_2(5)-1$

    Substitute into original terms to get common difference:

    $d=\log_5(2^x-\frac{1}{4})-\log_5(2^x+\frac{1}{2})$

    $\log_5(\frac{1}{2}-\frac{1}{4})-\log_5(\frac{1}{2}+\frac{1}{2})$ (substituting $2^x=\frac{1}{2})$

    $d=\log_5(\frac{1}{4})-\log_5(1)$

    $d=\log_5(\frac{1}{4})=\log_5(4^{-1})=-\log_5(4)$

    $\log_5(\frac{5}{2}-\frac{1}{4})-\log_5(\frac{5}{2}+\frac{1}{2})$ (substituting $2^x=\frac{5}{2})$

    $d=\log_5(\frac{9}{4})-\log_5(3)=\log_5(\frac{3}{4})$

    $d=\log_5(3)-\log_5(4)$

    \item 
    Start with equation 2:

    $\log_{10}\Bigl(\frac{x+y}{x-y}\Bigr)=\log_{10}(8)$

    $\frac{x+y}{x-y}=8$

    $x+y=8x-8y$

    $9y=7x$

    $y=\frac{7x}{9}$

    Substitute into equation 1:

    \(\log_{10}(x^2+(\frac{7x}{9})^2)=1+\log_{10}(13)\)

    \(\log_{10}\Bigl(x^2+(\frac{49x^2}{81})\Bigr)=1+\log_{10}(13)\)

    $\log_{10}\Bigl(\frac{130x^2}{81}\Bigr)=\log_{10}(10)+\log_{10}(13)$

    $\log_{10}\Bigl(\frac{130x^2}{81}\Bigr)=\log_{10}(130)$

    $\frac{130x^2}{81}=130$

    $\frac{x^2}{81}=1$

    $x^2=81$

    $x=\pm 9$

    Substitute into $y=\frac{7x}{9}$

    $y=7, -7$

    Solutions are $x=9, y=7$ and $x=-9, y=-7$

    However, we can't have a negative solution as $\log_{10}(-9--7)$ is undefined.

    Therefore, $x=9, y=7$


    \item 
    Evaluate the expression:

    \(\frac{1}{1+\log_a(bc)}+\frac{1}{1+\log_b(ac)}+\frac{1}{1+\log_c(ab)} \)

    Change everything to base 10:

    $\frac{1}{1+\frac{\log(bc)}{\log(a)}}+\frac{1}{1+\frac{\log(ac)}{\log(b)}}+\frac{1}{1+\frac{\log(ab)}{\log(c)}}$

    $\frac{1}{\frac{\log(a)+\log(bc)}{\log(a)}}+\frac{1}{\frac{\log(b)+\log(ac)}{\log(b)}}+\frac{1}{\frac{\log(c)+\log(ab)}{\log(c)}}$

    $\frac{\log(a)}{\log(a)+\log(bc)}+\frac{\log(b)}{\log(b)+\log(ac)}+\frac{\log(c)}{\log(c)+\log(ab)}$

    $\frac{\log(a)}{\log(a)+\log(b)+\log(c)}+\frac{\log(b)}{\log(b)+\log(a)+\log(c)}+\frac{\log(c)}{\log(c)+\log(a)+\log(b)}$

    $\frac{\log(a)+\log(b)+\log(c)}{\log(a)+\log(b)+\log(c)}=1$
\end{enumerate}




\end{document}